\documentclass[fleqn,12pt]{scrartcl}
\usepackage[utf8]{inputenc}
\usepackage{tikz}
\usepackage{color}
\usepackage[ngerman]{babel}
\usepackage{amssymb}
\usepackage{amsthm}
\usepackage{amsmath}
\usepackage{hyperref}
\usepackage{wasysym}
\usepackage{scrpage2}
\pagestyle{scrheadings}
\clearscrheadfoot
\ohead{\pagemark}
\ihead{Magnus Berendes, matrikelnr}
\ifoot{\today}
\ofoot{Blatt 3}
%\setheadtopline{1pt}
\setheadsepline{0.4pt}
\setfootsepline{0.4pt}
\usepackage{enumitem}
\setenumerate[0]{label=\alph*)}
\newcommand{\id}{\, \mathrm{d}}
\newcommand{\intl}{\int\displaylimits}
% New definition of square root:
% it renames \sqrt as \oldsqrt
\let\oldsqrt\sqrt
% it defines the new \sqrt in terms of the old one
\def\sqrt{\mathpalette\DHLhksqrt}
\def\DHLhksqrt#1#2{%
	\setbox0=\hbox{$#1\oldsqrt{#2\,}$}\dimen0=\ht0
	\advance\dimen0-0.2\ht0
	\setbox2=\hbox{\vrule height\ht0 depth -\dimen0}%
{\box0\lower0.4pt\box2}}

\newcommand{\karos}[2]{
	\begin{tikzpicture}
		\draw[step=0.5cm, color=gray] (0,0) grid (#1 cm , #2 cm);
	\end{tikzpicture}
}

\begin{document}
\section*{Blatt 3}
Bearbeitet/Zur Korrektur:

\noindent
\begin{Form}
	\CheckBox{Aufgabe A7}\\
	\CheckBox{Aufgabe A8}\\
	\CheckBox{Aufgabe A9}\\
	%\CheckBox{Aufgabe A4}
\end{Form}

\section{A7}
\begin{enumerate}
	\item
		\begin{align*}
			&f(x) = \cosh(x)\\
		 &P = \begin{pmatrix} 0\\1\end{pmatrix}\\
			&Q = \begin{pmatrix} \ln 5\\ \frac{13}5\end{pmatrix}
		\end{align*}

		\karos{10}{10}
	\item
		\begin{align*}
			\gamma(t) = \begin{pmatrix}
				t \\
				\cosh(t)
			\end{pmatrix}, t \in [0, \ln 5]
		\end{align*}

	\item
		\begin{align*}
			\text{Bogenl"ange } S &= \int\displaylimits_\gamma f(x) \id s = 
			\intl_0^{\ln5}\Vert\gamma'(t)\Vert \id t\\
		&= \intl_0^{\ln5} \left\Vert \begin{pmatrix} 1 \\ \sinh(t) \end{pmatrix} \right\Vert  \id t\\
		&= \intl_0^{\ln5}\sqrt{ 1 + \sinh^2(t)} \id t = \intl_0^{\ln5} \sqrt{\cosh^2(t)} \id t\\ 
		&= \left [
			\sinh(t)
		\right ]_0^{\ln5}\\
		&= \sinh(\ln5) - \sinh(0) = \frac{12}5
	\end{align*}

\item
	\begin{align*}
		g(x,y) =& \sinh(x) \sqrt{y}\\
		\intl_\gamma g \id s =& \intl_\gamma g \Vert \gamma'(t) \Vert \id t\\
		=& \intl_0^{4.5} \sinh(t) \sqrt{\cosh(t)}\cdot \cosh(t) \id t \\
		\underset{u:=\cosh(t)}=& \intl_1^{2.6}u^\frac32 \id u\\
		=& \left [ \frac25 u^\frac52 \right ]_1^{2.6} \approx 3.96
	\end{align*}

\end{enumerate}


\section{A8}
\begin{enumerate}
	\item
		\begin{align*}
		\gamma(t) &= \begin{pmatrix} t\\t-1\end{pmatrix}, t \in [0, 1], \gamma'(t) = \begin{pmatrix} 1\\ 1 \end{pmatrix} \\
		\id \vec s &= \gamma'(t) \id t\\
			W &= \intl_\gamma \vec F \cdot \id \vec s\\
		\vec F(x,& y) =  (x^2 + y^2) ^{-\frac32} \begin{pmatrix} x \\ y \end{pmatrix}\\
		\vec F(t,& t-1) = (t^2 + t^2 -2t + 1)^{-\frac32} \begin{pmatrix} t \\ t-1 \end{pmatrix}
		\end{align*}

		\begin{align*}
			W &= \intl_\gamma \vec F \cdot \id \vec s \\
				 &= \intl_0^1 \vec F(t, t-1) \cdot \gamma'(t) \id t\\
				 &= \intl_0^1 (t^2 + t^2 -2t + 1)^{-\frac32} \begin{pmatrix} t \\ t-1 \end{pmatrix} \cdot \begin{pmatrix}1\\1\end{pmatrix} \id t\\
				 &= \intl_0^1 (2t-1) (2t^2 -2t + 1)^{-\frac32} \id t\\
				 &\underset{u:=2t^2 -2t +1}{=} \intl_1^1 \frac{2t-1}{4t-2} \cdot u^{-\frac32}\id u \\
				 &= \frac12 \intl_1^1 u^{-\frac32} \id u = 0
		\end{align*}

	\item
		\begin{align*}
		\begin{pmatrix}0\\-1 \end{pmatrix} \rightarrow
		\begin{pmatrix}1 \\ -1 \end{pmatrix} \rightarrow
		\begin{pmatrix}1 \\ 0 \end{pmatrix}\\
		\end{align*}
		\begin{align*}
		\gamma_1(t_1) &= \begin{pmatrix} t_1\\ -1\end{pmatrix}, \gamma'_1(t_1) = \begin{pmatrix} 1\\ 0 \end{pmatrix}\\
		\gamma_2(t_2) &= \begin{pmatrix} 1 \\ t_2-1 \end{pmatrix}, \gamma'_2(t_2) = \begin{pmatrix} 0 \\ 1 \end{pmatrix}, t_{1,2} \in [0, 1] \\
			\gamma(t) &= \gamma_1(t_1) \cup \gamma_2(t_2)
		\end{align*}
		\begin{align*}
			W &= \intl_\gamma \vec F \id \vec s = \intl_{\gamma_1} \vec F \cdot \gamma_1'(t_1) \id t_1 + \intl_{\gamma_2} \vec F \cdot \gamma_2'(t_2) \id t_2 \\
				 &= \intl_0^1 \vec F(t_1, -1) \cdot \begin{pmatrix} 1\\0\end{pmatrix} \id t_1 +
		\intl_0^1 \vec F(1, t_2-1) \cdot \begin{pmatrix}0\\1\end{pmatrix} \id t_2\\
		&= \intl_0^1 (t_1^2 + 1)^{-\frac32} \begin{pmatrix} t_1 \\ -1 \end{pmatrix} \cdot \begin{pmatrix}1\\0\end{pmatrix} \id t_1+
		\intl_0^1(2 + t_2^2 - 2t_2)^{-\frac32} \begin{pmatrix}1\\t_2 -1\end{pmatrix} \cdot \begin{pmatrix} 0\\1\end{pmatrix} \id t_2\\
			&= \intl_0^1 t_1(t_1^2 + 1)^{-\frac32} \id t_1 + \intl_0^1 (t_2 -1)(2 + t_2^2 - 2t_2)^{-\frac32} \id t_2 \qquad| \substack{u:=t_1^2 + 1 \\ v:=2 + t_2^2 - 2t_2}\\
			&=\intl_1^2 \frac{t_1}{2t_1} \cdot u^{-\frac32} \id u +  \intl_2^1 \frac{t_2 -1}{2t_2 -2} \cdot v^{-\frac32} \id v \\
			&= \frac12 \cdot \left ( \left [-2 u^{-\frac12} \right ]_1^2 - \left [ -2v^{-\frac12} \right ]_1^2 \right ) = 0
		\end{align*}
	\item

		\begin{align*}
		\gamma(t) &= \begin{pmatrix}\sin(t)\\-\cos(t)\end{pmatrix}, t\in\left[0, \frac\pi2\right]\\
		\gamma'(t) &= \begin{pmatrix}\cos(t)\\ \sin(t) \end{pmatrix}
		\end{align*}
		\begin{align*}
		W &= \intl_0^\frac\pi2\vec F(\sin(t), -\cos(t)) \cdot \begin{pmatrix}\cos(t)\\\sin(t)\end{pmatrix} \id t\\
			 &= \intl_0^\frac\pi2 (\sin^2(t) + \cos^2(t))^{-\frac32} \begin{pmatrix}\sin(t)\\-\cos(t)\end{pmatrix} \cdot \begin{pmatrix} \cos(t)\\\sin(t)\end{pmatrix}\id t\\
			 &= \intl_0^\frac\pi2 \frac12 \sin(2t) - \frac12 \sin(2t) \id t = 0
		\end{align*}
\end{enumerate}

\section{A9}

\begin{enumerate}
	\item
		\begin{align*}
			O &= \intl_{I_1} \intl_{I_2} \left \Vert \partial_s \gamma(s,t) \times \partial_t \gamma(s, t)
			\right \Vert \id t \id s \\
			\gamma(\phi, h) &= \begin{pmatrix}
			\frac{Rh}{H} \cos \phi\\[0.3em]
			\frac{Rh}{H} \sin\phi\\[0.3em]
				h
			\end{pmatrix}
			\\
			\partial_\phi \gamma(\phi, h) &= \begin{pmatrix}
			\frac{Rh}{H} (-\sin \phi)\\[0.3em]
			\frac{Rh}{H} \cos\phi\\[0.3em]
				0
			\end{pmatrix}, \quad
			\partial_h \gamma(\phi, h) = \begin{pmatrix}
				\frac{R}{H} \cos \phi\\[0.3em]
			\frac{R}{H} \sin\phi\\[0.3em]
				1
			\end{pmatrix}\\
			\partial_\phi \gamma(\phi,h) \times \partial_h \gamma(\phi, h) &=
			\begin{pmatrix}
				\frac{Rh}H \cos \phi\\[0.3em]
				\frac{Rh}H \sin \phi\\[0.3em]
				\frac{Rh}H\cdot \frac{R}H \cdot (-\sin^2\phi - \cos^2\phi)
			\end{pmatrix}\\
			&= \frac{Rh}H \begin{pmatrix}
			\cos \phi\\[0.3em]
			\sin\phi\\[0.3em]
			-\frac{R}H
		\end{pmatrix}\\
\left \Vert \frac{Rh}H \begin{pmatrix}
			\cos \phi\\[0.3em]
			\sin\phi\\[0.3em]
			-\frac{R}H
		\end{pmatrix}\right \Vert &=
			\frac{Rh}H \cdot \sqrt{\cos^2\phi + \sin^2\phi+\frac{R^2}{H^2}} = \frac{Rh}H \cdot \sqrt{1 + \frac{R^2}{H^2}}
		\end{align*}
		\begin{align*}
			O(H, R) &= \intl_{I_1} \intl_{I_2} \left \Vert \partial_s \gamma(s,t) \times \partial_t \gamma(s, t)
			\right \Vert \id t \id s \\
			&= \intl_0^{2\pi} \intl_0^H \frac{Rh}H \cdot \sqrt{1+\frac{R^2}{H^2}} \id h \id \phi\\
			&= \intl_0^{2\pi} \frac{R}{2H} \cdot H^2 \cdot \sqrt{1+\frac{R^2}{H^2}} \id \phi\\
			&= \pi \cdot R \cdot \sqrt{H^2 +  R^2}
		\end{align*}
	\item

		\begin{align*}
			\intl_S \vec V \id \vec o &= \intl_{I_1} \intl_{I_2} \vec V(\gamma(s,t)) \cdot \left (\partial_s \gamma(s,t) \times \partial_t \gamma(s,t)\right) \id t \id s\\
																												 &= \intl_0^{2\pi} \intl_0^H \frac{Rh}H \cdot (\cos \phi + \sin \phi) \id h \id \phi \\
																												&= \intl_0^{2\pi} \frac12 H R (\cos \phi + \sin\phi) \id \phi \\
																											 &= \left [ \frac12 HR (-\sin \phi + \cos \phi) \right ]_0^{2\pi} = 0
		\end{align*}
\end{enumerate}

\end{document}
